Implement mixed-size access in UM promising model
- Msg.t: size as dependent record field (not type parameter), Ev.t = Msg.t
- Loc module removed, use address directly, Msg.loc renamed to Msg.addr
- GenPromising: add mEvent_eqb field and remove_dups_by
- VMPromising: decouple from UMPromising (own Loc, Msg, FwdItem)
- Remove sval/val aliases, use bv (8 * size) directly
- Add mixed-size Coq tests (STRW_LDRX, STRX_LDRW, MPmixed, MPmixedDMBS)
- Add mixed-size CLI litmus tests

ArchSemArm/VMPromising.v
@@ -43,8 +43,6 @@ From ASCommon Require Import Common GRel Exec FMon StateT HVec.
 From ArchSem Require Import GenPromising.
 Require Import ArmInst.
 
-Require UMPromising.
-Import (hints) UMPromising.
 
 #[local] Open Scope list.
 #[local] Open Scope nat.
@@ -53,14 +51,67 @@ Import (hints) UMPromising.
 (** The goal of this module is to define an Virtual memory promising model,
     without mixed-size on top of the new interface *)
 
-(** This model only works for 8-bytes aligned locations, as there
-    in no support for mixed-sizes yet. Also all location are
-    implicitly in the non-secure world.
+(** VM uses its own 8-byte-aligned Loc (bv 53), decoupled from
+    UMPromising.Loc which is now byte-granular for mixed-size. *)
+Module Loc.
+  Definition t := bv 53.
+  #[export] Typeclasses Transparent t.
+  #[export] Hint Transparent t : bv_unfold_db.
 
-    So in order to get the physical address you need to append 3 zeros.
+  #[global] Instance dec : EqDecision t.
+  Proof. unfold t. solve_decision. Defined.
 
-    We reuse the location setup from the User-Mode promising model. *)
-Module Loc := UMPromising.Loc.
+  Definition to_addr (loc : t) : address := bv_concat 56 loc (bv_0 3).
+
+  Definition from_addr (addr : address) : option t :=
+    if bv_extract 0 3 addr =? bv_0 3 then
+      Some (bv_extract 3 53 addr)
+    else None.
+
+  Lemma to_from_addr (addr : address) (loc : t) :
+    from_addr addr = Some loc → to_addr loc = addr.
+  Proof.
+    unfold from_addr,to_addr in *.
+    cdestruct addr,loc |- *** #CDestrMatch.
+    bv_solve'.
+  Qed.
+
+  Lemma from_to_addr (loc : t) : from_addr (to_addr loc) = Some loc.
+    unfold t in *.
+    unfold from_addr, to_addr.
+    cdestruct |- *** #CDestrMatch; bv_solve'.
+  Qed.
+
+  Definition to_addrs (loc : t) : list address := addr_range (to_addr loc) 8.
+
+  Definition from_addr_in (addr : address) : t := bv_extract 3 53 addr.
+
+  Definition addr_index (addr : address) : bv 3 := bv_extract 0 3 addr.
+
+  Lemma from_addr_addr_in addr loc :
+    from_addr addr = Some loc → from_addr_in addr = loc.
+  Proof. unfold from_addr,from_addr_in. cdestruct |- *** #CDestrMatch. Qed.
+
+  Lemma from_addr_in_to_addrs loc :
+    ∀ addr ∈ to_addrs loc, from_addr_in addr = loc.
+  Proof.
+    unfold from_addr_in, to_addrs, addr_range, addr_addN, to_addr.
+    set_unfold.
+    cdestruct |- ***.
+    unfold t, addr_size in *.
+    bv_solve.
+  Qed.
+
+  Definition to_va (loc : t) : bv 64 :=
+    bv_concat 64 (bv_0 8) $ bv_concat 52 loc (bv_0 3).
+
+  Definition from_va (addr : bv 64) : option t :=
+    if bv_extract 0 3 addr =? bv_0 3 then
+      Some (bv_extract 3 53 addr)
+    else None.
+
+End Loc.
+Export (hints) Loc.
 
 (** Register and memory values (all memory access are 8 bytes aligned *)
 Definition val := bv 64.
@@ -69,8 +120,27 @@ Definition val := bv 64.
 Definition val_to_address (v : val) : address :=
   bv_extract 0 56 v.
 
-(** We also reuse the Msg object from the User-Mode Promising Model. *)
-Module Msg := UMPromising.Msg.
+(** VM uses its own fixed-size Msg (8-byte aligned, no mixed-size).
+    Decoupled from UMPromising.Msg which supports mixed-size access. *)
+Module Msg.
+  Record t :=
+    make {
+      tid : nat;
+      loc : Loc.t;
+      val : val;
+    }.
+  Arguments make : clear implicits.
+
+  #[global] Instance eq_dec : EqDecision t.
+  Proof. solve_decision. Defined.
+
+  #[global] Instance count : Countable t.
+  Proof.
+    apply (inj_countable' (λ msg, (tid msg, loc msg, val msg))
+                      (λ x, make x.1.1 x.1.2 x.2)).
+    by intros [].
+  Defined.
+End Msg.
 
 Module TLBI.
   Inductive t :=
@@ -142,6 +212,8 @@ Module Ev.
   #[global] Instance dec : EqDecision t.
   solve_decision.
   Defined.
+
+  Definition eqb (e1 e2 : t) : bool := bool_decide (e1 = e2).
 
   Definition tid (ev : t) :=
     match ev with
@@ -333,7 +405,15 @@ Module Memory.
 End Memory.
 Import (hints) Memory.
 
-Module FwdItem := UMPromising.FwdItem.
+Module FwdItem.
+  Record t :=
+    make {
+      time : nat;
+      view : view;
+      xcl : bool
+    }.
+  Definition init := make 0 0 false.
+End FwdItem.
 
 
 Definition EL := (fin 4).
@@ -1734,7 +1814,11 @@ Module IIS.
 
 End IIS.
 
-Import UMPromising(view_if, read_fwd_view).
+Definition view_if (b : bool) (v : view) := if b then v else 0%nat.
+
+Definition read_fwd_view (macc : mem_acc) (f : FwdItem.t) :=
+  if f.(FwdItem.xcl) && is_rel_acq macc
+  then f.(FwdItem.time) else f.(FwdItem.view).
 
 (** Perform an explicit memory read.
 
@@ -2504,6 +2588,7 @@ Definition VMPromising (bbm_param : BBM.param) : Promising.Model :=
     iis_init := IIS.init;
     address_space := PAS_NonSecure;
     mEvent := Ev.t;
+    mEvent_eqb := Ev.eqb;
     mEvent_tid := Ev.tid;
     handle_outcome := run_outcome;
     emit_promise := λ tid initmem mem msg, TState.promise (length mem);
